init/uninit and illegal accesses

ByteArray.v
@@ -6,569 +6,341 @@ From MyProject Require Import Integers.
 From MyProject Require Import Maps.
 From MyProject Require Import ListUtils.
 From MyProject Require Import CrVarLike.
+From MyProject Require Import CrVal.
+From MyProject Require Import SmtExpr.
+From MyProject Require Import SmtTypes.
+From MyProject Require Import SmtQuery.
 
 (*
 In essence, I'm representing memory as a set of arrays.
 Each array boils down to a starting address, a length, and the bytes themselves.
 *)
-Record Array := {
-  base : nat;
-  len : nat;
-  bytes : PMap.t (option uint8)
-}.
-Definition Memory := PMap.t (option Array).
 
+(* explicit uninitialized data type *)
 (*
-Because bytes are stored as a PMap.t, each byte is associated with
-a positive number. I'm doing 0-indexing, so that means that index i
-is a natural number (incl. 0), but the key in the PMap associated
-with it is i + 1 (since 0 \notin positive).
+error return type(?)
+- affects notion of transformation validity
+
+eBPF
+- Possibly assume program passes checker
+
+Make a prop + proof that assumes program accesses are in bounds.
+
+for the states that wouldn't generate an error...
 *)
+
+(* An array is an allocated block of contiguous memory *)
+(* Said block has an associated length *)
+Inductive LookupVal {T : Type} :=
+| Init (v : T)
+| Uninit.
+Record MemBlock (T : Type) := {
+  arr_len : positive;
+  arr_bytes : PMap.t (@LookupVal T);
+}.
+Arguments arr_len {T} _.
+Arguments arr_bytes {T} _.
+Inductive Array {T : Type} :=
+| Allocated (arr : MemBlock T)
+| Unallocated.
+Arguments Unallocated {T}.
+Inductive Check_T (T : Type) :=
+| Legal (v : T)
+| Illegal.
+Arguments Legal {T} _.
+Arguments Illegal {T}.
+
+(* A program's memory is a collection of arrays *)
+Definition Memory (T : Type) := PMap.t (@Array T).
+Record MachineState (T : Type) := {
+  reg_state : PMap.t T;
+  mem_state : Memory T;
+}.
+Arguments reg_state {T} _.
+Arguments mem_state {T} _.
+
+(* Values in the array can either be initialized or not *)
+Definition ConcreteMState := MachineState CrVal.
+Definition SymbolicMState := MachineState SmtArithExpr.
+
 Definition keys_from_map {T : Type} (m : PMap.t T) : list positive :=
   List.map fst (PTree.elements (snd m)).
-Definition key_to_idx (k: positive) : nat :=
-  (Pos.to_nat k) - 1.
-Definition idx_to_key (i: nat) : positive :=
-  (Pos.of_nat (i + 1)).
-
-(* more map accessor helpers since I'm storing an option type *)
+Transparent keys_from_map.
 Definition vals_from_map {T : Type} (m : PMap.t T) : list T :=
   List.map snd (PTree.elements (snd m)).
-Fixpoint unnone {T : Type} (l : list (option T)) : list T :=
-  match l with
-  | [] => []
-  | x :: xs => match x with
-    | Some x' => x' :: (unnone xs)
-    | None => unnone xs
+Transparent vals_from_map.
+
+Definition block_is_valid {T : Type} (block : MemBlock T) : Prop :=
+  forall (idx : positive),
+  PTree.get idx (snd (arr_bytes block)) <> None -> (Pos.le idx (arr_len block)).
+
+Definition Mt {T : Type} (len : positive) : MemBlock T := {|
+  arr_len := len;
+  arr_bytes := PMap.init Uninit;
+|}.
+Definition TabulaRasa {T : Type} : Memory T :=
+  PMap.init Unallocated.
+
+Lemma mt_is_valid:
+  forall (T: Type) (len : positive),
+  @block_is_valid T (Mt len).
+Proof.
+  unfold block_is_valid.
+  intros.
+  unfold Mt. simpl in *.
+  unfold PTree.get in H. simpl in H.
+  exfalso. congruence.
+Qed.
+
+Definition get_array {T : Type} (mem : Memory T) (base : positive) : Array :=
+  mem !! base.
+Transparent get_array.
+
+Definition mem_disjoint {T : Type} (mem : Memory T) : Prop :=
+  forall (base base' : positive),
+  Pos.lt base base' ->
+  match get_array mem base, get_array mem base' with
+  | Allocated block, Allocated block' =>
+    let len := arr_len block in
+    let len' := arr_len block' in
+    Pos.le (Pos.add base len) base'
+  | _, _ => True
+  end.
+
+Definition mem_is_valid {T : Type} (mem : Memory T) : Prop :=
+  mem_disjoint mem /\ (
+    forall (base : positive),
+    match get_array mem base with
+    | Allocated block => block_is_valid block
+    | Unallocated => True
     end
-  end.
-Definition vals_from_map' {T : Type} (m : PMap.t (option T)) : list T :=
-  unnone (vals_from_map m).
+  ).
 
-(* checks that two arrays don't overlap *)
-Definition arrays_disjoint (a1 a2 : Array) : bool :=
-  let start1 := base a1 in
-  let end1 := (base a1) + (len a1) in
-  let start2 := base a2 in
-  let end2 := (base a2) + (len a2) in
-  (negb (start1 =? start2)) && (
-    ((start1 <? start2) && (end1 <? start2)) ||
-    ((start2 <? start1) && (end2 <? start1))).
-(* checks that an array doesn't overlap with any other arrays *)
-Definition array_unique (x : Array) (xs : list Array) :=
-  List.forallb (fun x' => arrays_disjoint x x') xs.
-Fixpoint mem_disjoint_helper (A : list Array) :=
-  match A with
-  | [] => true
-  | x :: xs => if (array_unique x xs) then
-      mem_disjoint_helper xs
+Lemma tab_rasa_is_valid:
+  forall (T : Type),
+  mem_is_valid (@TabulaRasa T).
+Proof.
+  unfold mem_is_valid, mem_disjoint. split;
+  intros; simpl;
+  apply I.
+Qed.
+
+(* load the value that a pointer points to *)
+Definition ld_block {T : Type} (block : MemBlock T) (idx : positive) : @LookupVal T :=
+  (arr_bytes block) !! idx.
+Definition ld_mem {T : Type} (mem : Memory T) (base : positive) (idx : positive)
+  : Check_T LookupVal :=
+  match (get_array mem base) with
+  | Allocated block => Legal (ld_block block idx)
+  | Unallocated => Illegal
+  end.
+
+(* store a value into a pointer *)
+Definition st_block {T : Type} (block : MemBlock T) (idx : positive) (v : T) : MemBlock T := {|
+  arr_len := arr_len block;
+  arr_bytes := PMap.set idx (Init v) (arr_bytes block);
+|}.
+Definition st_mem {T : Type} (mem : Memory T) (base : positive) (idx : positive) (v : T) : Check_T (Memory T) :=
+  match (get_array mem base) with
+  | Allocated block =>
+    let block_len := arr_len block in
+    if (Pos.leb idx block_len) then
+      let block' := st_block block idx v in
+      Legal (PMap.set base (Allocated block') mem)
     else
-      false
+      Illegal
+  | Unallocated => Illegal
   end.
-(* checks that all arrays are unique *)
-Definition memory_disjoint (mem : Memory) : bool :=
-  mem_disjoint_helper (vals_from_map' mem).
 
-Fixpoint valid_offset_helper (off : list nat) (len : nat) :=
-  match off with
-  | [] => true
-  | x :: xs => andb (x <? len) (valid_offset_helper xs len)
+Lemma ltb_neq:
+  forall (x y : positive),
+  Pos.lt x y -> x <> y.
+Proof.
+  intros.
+  intro Hc. rewrite Hc in H.
+  specialize Pos.lt_irrefl with (x := y).
+  intros. congruence.
+Qed.
+
+Ltac b_to_props :=
+  repeat match goal with
+  | H : (?x =? ?y)%positive = true |- _ =>
+    apply Pos.eqb_eq in H
+  | H : (?x =? ?y)%positive = false |- _ =>
+    apply Pos.eqb_neq in H
   end.
-(* checks that an array has no out-of-bounds stores *)
-Definition has_valid_offsets (a : Array) : bool :=
-  let l := len a in
-  let mem := bytes a in
-  let idxs := List.map key_to_idx (keys_from_map mem) in
-  valid_offset_helper idxs l.
-(* checks that all arrays have no OoB stores *)
-Definition all_array_offsets_valid (mem : Memory) : bool :=
-  List.forallb has_valid_offsets (vals_from_map' mem).
 
-(* what I'm initially assuming to be a sane understanding of valid memory *)
-Definition valid_memory (mem : Memory) : Prop :=
-  (* arrays have different address ranges *)
-  ((memory_disjoint mem) = true) /\
-  (* arrays stay within their address ranges *)
-  ((all_array_offsets_valid mem) = true).
+Lemma st_mem_preserves_validity:
+  forall (T : Type) (mem : Memory T) (base : positive) (idx : positive) (v : T),
+  mem_is_valid mem -> match (st_mem mem base idx v) with
+  | Legal mem' => mem_is_valid mem'
+  | Illegal => True
+  end.
+Proof with try assumption; try apply I.
+  intros. unfold mem_is_valid in *.
+  destruct (st_mem mem base idx v) eqn:Hst...
+  split.
+  admit.
+Admitted.
+
+(* Memory-capable IR *)
+Inductive FnArg {T : Type} : Type :=
+| PosArg (p : positive)
+| RegArg (r : positive)
+| ValArg (v : T).
+
+Inductive Op {T : Type} : Type :=
+| Alloc (arg1 arg2 : @FnArg T)
+| Assign (arg1 arg2 : @FnArg T)
+| Ld (arg1 arg2 : @FnArg T)
+| St (arg1 arg2 : @FnArg T)
+| Add (arg1 arg2 : @FnArg T).
+
+Definition Program {T : Type} : Type := list (@Op T).
+
+Definition alloc {T : Type} (m : MachineState T) (arg1 arg2 : @FnArg T) : Check_T (MachineState T) :=
+  match arg1, arg2 with
+  | PosArg b, PosArg l => Legal {|
+    reg_state := reg_state m;
+    mem_state := PMap.set b (Allocated {|
+      arr_len := l;
+      arr_bytes := PMap.init Uninit;
+    |}) (mem_state m);
+  |}
+  | _, _ => Illegal
+  end.
+
+Definition set_reg {T : Type} (m : MachineState T) (arg1 arg2 : @FnArg T) : Check_T (MachineState T) :=
+  match arg1, arg2 with
+  | RegArg dst, RegArg src => Legal {|
+    reg_state := PMap.set dst ((reg_state m) !! src) (reg_state m);
+    mem_state := mem_state m;
+  |}
+  | RegArg dst, ValArg v => Legal {|
+    reg_state := PMap.set dst v (reg_state m);
+    mem_state := mem_state m;
+  |}
+  | _, _ => Illegal
+  end.
 
 Definition uint_to_pos (u : uintptr) : positive :=
   Pos.of_nat ((Z.to_nat (unsigned u)) + 1).
 
-(* check if a pointer's array is in memory *)
-Definition find_array (mem : Memory) (base : uintptr) : option Array :=
-  mem !! (uint_to_pos base).
-
-(* load the value that a pointer points to *)
-Definition ld_arr (a : Array) (offset : uintptr) : option uint8 :=
-  let offset' := uint_to_pos offset in
-  if (Pos.ltb offset' (Pos.of_nat (len a))) then
-     (bytes a) !! offset'
-  else
-    None.
-Definition ld_mem (mem : Memory) (base : uintptr) (offset : uintptr) : option uint8 :=
-  match (find_array mem base) with
-  | Some a => ld_arr a offset
-  | None => None
-  end.
-
-(* store a value into a pointer *)
-Definition st_arr (a : Array) (offset : uintptr) (v : uint8) : option Array :=
-  let offset' := uint_to_pos offset in
-  if (Pos.ltb offset' (Pos.of_nat (len a))) then
-    Some {|
-      base := base a;
-      len := len a;
-      bytes := PMap.set offset' (Some v) (bytes a)
-    |}
-  else
-    None.
-Definition st_mem' (mem : Memory) (base : uintptr) (offset : uintptr) (v : uint8) : option Memory :=
-  match (find_array mem base) with
-  | Some a => match (st_arr a offset v) with
-    | Some a' => Some (PMap.set (uint_to_pos base) (Some a') mem)
-    | None => None
-    end
-  | None => None
-  end.
-Definition st_mem (mem : Memory) (base : uintptr) (offset : uintptr) (v : uint8) : Memory :=
-  match (st_mem' mem base offset v) with
-  | Some mem' => mem'
-  | None => mem
-  end.
-
-(* accessing a pointer is valid if...
-  - there exists an associated array in memory
-  - the pointer's access into that array is in-bounds *)
-Definition mem_access_valid (mem: Memory) (base : uintptr) (offset : uintptr) : Prop :=
-  let a := find_array mem base in
-  let l := match a with
-  | Some a' => (Pos.of_nat (len a'))
-  | None => 1%positive
-  end in
-  (a <> None) /\ ((Pos.ltb (uint_to_pos offset) l) = true).
-
-(* random lemma I felt like proving *)
-Ltac isi := intros; split; intros.
-Lemma valid_st_lemma:
-  forall (mem : Memory) (base : uintptr) (offset : uintptr) (v : uint8),
-  mem_access_valid mem base offset <->
-  (st_mem' mem base offset v) <> None.
-Proof.
-  isi.
-  - destruct H as [Ha Ho].
-    unfold st_mem'.
-    destruct (find_array mem base0); try (exfalso; congruence).
-    unfold st_arr. rewrite Ho. discriminate.
-  - unfold mem_access_valid.
-    unfold st_mem' in H.
-    destruct (find_array mem base0); try (exfalso; congruence).
-    split; try discriminate.
-    destruct (Pos.ltb (uint_to_pos offset) (Pos.of_nat (len a))) eqn:Hlt; try reflexivity.
-    unfold st_arr in H.
-    rewrite Hlt in H.
-    exfalso. congruence.
-Qed.
-
-Lemma still_valid_lemma:
-  forall (mem : Memory) (base : uintptr) (offset : uintptr) (v : uint8),
-  mem_access_valid mem base offset <->
-  mem_access_valid (st_mem mem base offset v) base offset.
-Proof.
-  isi; unfold mem_access_valid in *; destruct H as [Ha Ho].
-  - split; unfold st_mem, st_mem';
-    destruct (find_array mem base0); try congruence;
-    unfold st_arr;
-    rewrite Ho; unfold find_array;
-    rewrite PMap.gss; try discriminate.
-    simpl. assumption.
-  - split.
-    + unfold st_mem, st_mem' in *.
-      destruct (find_array mem base0) eqn:Hp; try congruence.
-    + unfold st_mem, st_mem' in *.
-      destruct (find_array mem base0) eqn:Hp.
-      * destruct (st_arr a offset v) eqn:Hst.
-      -- destruct (find_array (PMap.set (uint_to_pos base0) (Some a0) mem) base0) eqn:Ha1.
-      ++ unfold find_array in Ha1.
-         rewrite PMap.gss in Ha1.
-         injection Ha1 as Ha1.
-         rewrite <- Ha1 in Ho.
-         unfold st_arr in Hst.
-         destruct ((uint_to_pos offset <? Pos.of_nat (len a))%positive); try reflexivity.
-         exfalso. congruence.
-      ++ exfalso. congruence.
-      -- rewrite Hp in Ho. assumption.
-      * rewrite Hp in Ho. assumption.
-Qed.
-
-(* read after write lemmas *)
-Lemma raw_same_address:
-  forall (mem : Memory) (base : uintptr) (offset : uintptr) (v : uint8),
-  mem_access_valid mem base offset <->
-  ld_mem (st_mem mem base offset v) base offset = Some v.
-Proof with try congruence.
-  intros; split; intros.
-  - assert (mem_access_valid (st_mem mem base0 offset v) base0 offset). {
-      apply still_valid_lemma. assumption.
-    }
-    destruct H as [Ha Ho].
-    destruct H0 as [Ha' Ho'].
-    destruct (find_array mem base0) eqn:Hp...
-    destruct (find_array (st_mem mem base0 offset v) base0) eqn:Hp'...
-    unfold ld_mem.
-    destruct (find_array (st_mem mem base0 offset v) base0) eqn:Hp''...
-    unfold ld_arr.
-    injection Hp' as Hp'. rewrite Hp'.
-    destruct ((uint_to_pos offset <? Pos.of_nat (len a0))%positive)...
-    rewrite Hp' in Hp''.
-    unfold find_array in Hp''.
-    unfold st_mem, st_mem' in Hp''.
-    rewrite Hp in Hp''.
-    unfold st_arr in Hp''.
-    rewrite Ho in Hp''.
-    rewrite PMap.gss in Hp''.
-    injection Hp'' as Hp''.
-    rewrite <- Hp''. simpl.
-    rewrite PMap.gss. reflexivity.
-  - unfold mem_access_valid. split.
-    + unfold ld_mem in H.
-      destruct (find_array mem base0) eqn:Hp...
-      unfold st_mem, st_mem' in H.
-      repeat rewrite Hp in H.
-      exfalso. congruence.
-    + unfold ld_mem, ld_arr in H.
-      unfold st_mem, st_mem', st_arr in H.
-      destruct (find_array mem base0) eqn:Hp.
-      * destruct ((uint_to_pos offset <? Pos.of_nat (len a))%positive) eqn:Ho...
-        rewrite Hp in H.
-        rewrite Ho in H.
-        exfalso. congruence.
-      * rewrite Hp in H. exfalso. congruence.
-Qed.
-Lemma raw_different_address:
-  forall (mem : Memory) (b1 b2 : uintptr) (o1 o2 : uintptr) (v : uint8),
-  (o1 <> o2 \/ b1 <> b2) ->
-  ld_mem mem b1 o1 = ld_mem (st_mem mem b2 o2 v) b1 o1.
-Proof with try congruence; try discriminate; try reflexivity.
-  intros.
-  unfold st_mem, st_mem'.
-  destruct (find_array mem b2) eqn:Hp2...
-  destruct (st_arr a o2 v) eqn:Ha2'...
-  unfold ld_mem, find_array.
-  destruct H.
-  - unfold st_arr in Ha2'.
-    destruct (Pos.ltb (uint_to_pos o2) (Pos.of_nat (len a))) eqn:Hltb...
-    injection Ha2' as Ha2'.
-    destruct (Pos.eq_dec (uint_to_pos b1) (uint_to_pos b2)) as [Hbeq | Hbneq].
-    + repeat rewrite Hbeq. rewrite PMap.gss.
-      unfold find_array in Hp2.
-      rewrite Hp2.
-      unfold ld_arr.
-      rewrite <- Ha2'; simpl.
-      rewrite PMap.gso...
-      unfold uint_to_pos.
-      admit.
-      (* intro Heq.
-      apply Nat2Pos.inj in Heq.
-      * unfold Z.to_nat in Heq.
-        destruct  *)
-    + rewrite PMap.gso...
-  - rewrite PMap.gso...
-    admit.
-Admitted.
-
-(* Toy Grammar *)
-(* Values *)
-From MyProject Require Import CrVal.
-Inductive RegArg : Type :=
-| Reg (x : positive).
-Definition reg' (r : RegArg) : positive :=
-  match r with
-  | Reg x => x
-  end.
-
-(* Operators *)
-Inductive Op : Type :=
-  (*  *)
-  (* creates an array in memory *)
-| Alloc (base nbyte : nat)
-  (* dst_reg = v *)
-| SetVal (dst_reg : RegArg) (v : CrVal)
-  (* dst_reg = src_reg *)
-| SetReg (dst_reg src_reg : RegArg)
-  (* dst_reg = *src_reg *)
-| LdReg (dst_reg src_reg : RegArg)
-  (* *dst_reg = v *)
-| StVal (dst_reg : RegArg) (v : CrVal)
-  (* *dst_reg = src_reg *)
-| StReg (dst_reg src_reg : RegArg)
-  (* *dst_reg = *src_reg *)
-| IStReg (dst_reg src_reg : RegArg)
-  (* dst_reg = src_reg + v *)
-| AddVal (dst_reg src_reg : RegArg) (v : CrVal)
-  (* dst_reg = src_reg1 + src_reg2 *)
-| AddReg (dst_reg src_reg1 src_reg2 : RegArg).
-
-Record MachineState := {
-  reg_state : PMap.t CrVal;
-  mem_state : Memory;
-}.
-
-Definition Interp : Type :=
-  MachineState -> MachineState.
-Definition Program : Type :=
-  list Op.
-
-Definition get_reg (m : MachineState) (r : RegArg) : CrVal :=
-  (reg_state m) !! (reg' r).
-Transparent get_reg.
-Definition x_reg (m : MachineState) (r : RegArg) : CrVal :=
-  match get_reg m r with
-  | CrPtr b o =>
-    match ld_mem (mem_state m) b o with
-    | Some v => CrInt v
-    | None => CrNil
-    end
-  | _ => CrNil
-  end.
-Transparent x_reg.
-Definition alloc (base nbyte : nat) (m : MachineState) : MachineState := {|
-  reg_state := reg_state m;
-  mem_state := PMap.set (Pos.of_nat (base+1)) (Some {|
-    base := base;
-    len := nbyte;
-    bytes := PMap.init None
-  |}) (mem_state m);
-|}.
-Transparent alloc.
-Definition set_val (dst_reg : RegArg) (v : CrVal) (m : MachineState) : MachineState := {|
-  reg_state := PMap.set (reg' dst_reg) v (reg_state m);
-  mem_state := mem_state m;
-|}.
-Transparent set_val.
-Definition set_reg (dst_reg src_reg : RegArg) (m : MachineState) : MachineState := {|
-  reg_state := PMap.set (reg' dst_reg) ((reg_state m) !! (reg' src_reg)) (reg_state m);
-  mem_state := mem_state m;
-|}.
-Definition ld_reg (dst_reg src_reg : RegArg) (m : MachineState) : MachineState :=
-  let ld_val := x_reg m src_reg in {|
-  reg_state := PMap.set (reg' dst_reg) ld_val (reg_state m);
-  mem_state := mem_state m;
-|}.
-Transparent ld_reg.
-Definition st_val (dst_reg : RegArg) (v : CrVal) (m : MachineState) : MachineState :=
-  match (reg_state m) !! (reg' dst_reg), v with
-  | CrPtr b o, CrInt x => {|
-      reg_state := reg_state m;
-      mem_state := st_mem (mem_state m) b o x;
-    |}
-  | _, _ => m
-  end.
-Transparent st_val.
-Definition st_reg (dst_reg src_reg : RegArg) (m : MachineState) : MachineState :=
-  match (reg_state m) !! (reg' dst_reg), (reg_state m) !! (reg' src_reg) with
-  | CrPtr b o, CrInt x => {|
-      reg_state := reg_state m;
-      mem_state := st_mem (mem_state m) b o x;
-    |}
-  | _, _ => m
-  end.
-Transparent st_reg.
-Definition ist_reg (dst_reg src_reg : RegArg) (m : MachineState) : MachineState :=
-  match (reg_state m) !! (reg' dst_reg), (reg_state m) !! (reg' src_reg) with
-  | CrPtr b' o', CrPtr b o => match ld_mem (mem_state m) b o with
-    | Some v => {|
-        reg_state := reg_state m;
-        mem_state := st_mem (mem_state m) b' o' v;
+Definition ld_reg' (m : ConcreteMState) (arg1 arg2 : @FnArg CrVal) : Check_T (ConcreteMState) :=
+  match arg1, arg2 with
+  | RegArg dst, RegArg src =>
+    match (reg_state m) !! src with
+    | CrPtr b o =>
+      match ld_mem (mem_state m) (uint_to_pos b) (uint_to_pos o) with
+      | Legal (Init v) => Legal {|
+        reg_state := PMap.set dst v (reg_state m);
+        mem_state := mem_state m;
       |}
-    | None => m
+      | _ => Illegal
+      end
+    | _ => Illegal
     end
-  | _, _ => m
+  | RegArg dst, ValArg (CrPtr b o) =>
+    match ld_mem (mem_state m) (uint_to_pos b) (uint_to_pos o) with
+    | Legal (Init v) => Legal {|
+      reg_state := PMap.set dst v (reg_state m);
+      mem_state := mem_state m;
+    |}
+    | _ => Illegal
+    end
+  | _, _ => Illegal
   end.
-Transparent ist_reg.
-Definition add_val (dst_reg src_reg : RegArg) (v : CrVal) (m : MachineState) : MachineState :=
-  set_val dst_reg match (reg_state m) !! (reg' src_reg), v with
-  | CrInt x, CrInt y => CrInt (Integers.add x y)
-  | CrPtr x y, CrInt z =>
-    let z' : uintptr := repr (intval z) in
-    CrPtr x (Integers.add y z')
-  | _, _ => CrNil
-  end m.
-Transparent add_val.
-Definition add_reg (dst_reg src_reg1 src_reg2 : RegArg) (m : MachineState) : MachineState :=
-  set_val dst_reg match (reg_state m) !! (reg' src_reg1), (reg_state m) !! (reg' src_reg2) with
-  | CrInt x, CrInt y => CrInt (Integers.add x y)
-  | CrPtr x y, CrInt z =>
-    let z' : uintptr := repr (intval z) in
-    CrPtr x (Integers.add y z')
-  | _, _ => CrNil
-  end m.
-Transparent add_reg.
 
-Definition apply_op (op : Op) (m : MachineState) : MachineState :=
+Definition st_reg' (m : ConcreteMState) (arg1 arg2 : @FnArg CrVal) : Check_T (ConcreteMState) :=
+  match arg1, arg2 with
+  | RegArg dst, RegArg src =>
+    match (reg_state m) !! dst, (reg_state m) !! src with
+    | CrPtr b o, v =>
+      match st_mem (mem_state m) (uint_to_pos b) (uint_to_pos o) v with
+      | Legal mem' => Legal {|
+        reg_state := reg_state m;
+        mem_state := mem';
+      |}
+      | _ => Illegal
+      end
+    | _, _ => Illegal
+    end
+  | RegArg dst, ValArg v =>
+    match (reg_state m) !! dst with
+    | CrPtr b o =>
+      match st_mem (mem_state m) (uint_to_pos b) (uint_to_pos o) v with
+      | Legal mem' => Legal {|
+        reg_state := reg_state m;
+        mem_state := mem';
+      |}
+      | _ => Illegal
+      end
+    | _ => Illegal
+    end
+  | _, _ => Illegal
+  end.
+
+Definition add_reg' (m : ConcreteMState) (arg1 arg2 : @FnArg CrVal) : Check_T (ConcreteMState) :=
+  match arg1, arg2 with
+  | RegArg dst, RegArg src =>
+    match (reg_state m) !! dst, (reg_state m) !! src with
+    | CrInt x, CrInt y => Legal {|
+        reg_state := PMap.set dst (CrInt (Integers.add x y)) (reg_state m);
+        mem_state := mem_state m;
+      |}
+    | CrPtr b o, CrInt y =>
+      let y' : uintptr := repr (intval y) in
+      Legal {|
+        reg_state := PMap.set dst (CrPtr b (Integers.add o y')) (reg_state m);
+        mem_state := mem_state m;
+      |}
+    | _, _ => Illegal
+    end
+  | RegArg dst, ValArg v =>
+    match (reg_state m) !! dst, v with
+    | CrInt x, CrInt y => Legal {|
+        reg_state := PMap.set dst (CrInt (Integers.add x y)) (reg_state m);
+        mem_state := mem_state m;
+      |}
+    | CrPtr b o, CrInt y =>
+      let y' : uintptr := repr (intval y) in
+      Legal {|
+        reg_state := PMap.set dst (CrPtr b (Integers.add o y')) (reg_state m);
+        mem_state := mem_state m;
+      |}
+    | _, _ => Illegal
+    end
+  | _, _ => Illegal
+  end.
+
+Definition example_program : Program := [
+  Alloc  (PosArg 1) (PosArg 1024); (* allocate 1024 bytes at base 1 *)
+  Assign (RegArg 2) (ValArg (CrPtr (repr 1) (repr 0))); (* r2 = ptr to base 1, offset 0 *)
+  St     (RegArg 2) (ValArg (CrInt (repr 42))); (* *r2 = 42 *)
+  Ld     (RegArg 3) (RegArg 2); (* r3 = *r2 *)
+  Add    (RegArg 4) (RegArg 3) (* r4 = r3 + r3 *)
+].
+
+Definition apply_concrete (op : Op) (m : ConcreteMState) : Check_T ConcreteMState :=
   match op with
-  | Alloc b n => alloc b n
-  | SetVal d v => set_val d v
-  | SetReg d s => set_reg d s
-  | LdReg d s => ld_reg d s
-  | StVal d v => st_val d v
-  | StReg d s => st_reg d s
-  | IStReg d s => ist_reg d s
-  | AddVal d s v => add_val d s v
-  | AddReg d s1 s2 => add_reg d s1 s2
-  end m.
-
-Fixpoint compile' (p : Program) (m : MachineState) : MachineState :=
-  match p with
-  | [] => m
-  | x :: xs => compile' xs (apply_op x m)
+  | Alloc arg1 arg2 => alloc m arg1 arg2
+  | Assign arg1 arg2 => set_reg m arg1 arg2
+  | Ld arg1 arg2 => ld_reg' m arg1 arg2
+  | St arg1 arg2 => st_reg' m arg1 arg2
+  | Add arg1 arg2 => add_reg' m arg1 arg2
   end.
-Definition compile (p : Program) : Interp :=
-  compile' p.
 
-From MyProject Require Import SmtExpr.
-Definition check_registers_and_memory (s1 s2 : MachineState)
-  (reg_list : list RegArg) (mem_list : list (uintptr * uintptr)) : SmtBoolExpr :=
-  SmtBoolNot (SmtBoolAnd
-    (List.fold_right
-      (fun r acc => SmtBoolAnd acc (SmtBoolEq
-        (SmtConst (get_reg s1 r))
-        (SmtConst (get_reg s2 r))))
-      SmtTrue reg_list)
-    (List.fold_right (fun p acc =>
-      SmtBoolAnd acc (match p with
-      | (base, offset) =>
-        SmtBoolEq
-          (match ld_mem (mem_state s1) base offset with
-          | Some v => SmtConst (CrInt v)
-          | None => SmtConst CrNil
-          end)
-          (match ld_mem (mem_state s2) base offset with
-          | Some v => SmtConst (CrInt v)
-          | None => SmtConst CrNil
-          end)
-      end))
-      SmtTrue mem_list)
-  ).
-
-From MyProject Require Import SmtTypes.
-From MyProject Require Import SmtQuery.
-Definition eq_checker (s : MachineState)
-  (p1 p2 : Program)
-  (reg_list : list RegArg) (mem_list : list (uintptr * uintptr)) : SmtResult :=
-  let s1 := compile p1 s in
-  let s2 := compile p2 s in
-  smt_query (check_registers_and_memory s1 s2 reg_list mem_list).
-
-Record ProgramOutput := {
-  out_reg : list RegArg;
-  out_mem : list Ptr;
-}.
-
-Definition get_output (p : Program) (o : ProgramOutput) (m : MachineState) : list Value * list Value :=
-  let m' := (compile p) m in
-  (* for each number in (out_reg o), map get_reg onto m' *)
-  let reg_vals := List.map (fun r => (reg_state m') !! (reg' r)) (out_reg o) in
-  let mem_vals := List.map (fun p =>
-    match ld_mem (mem_state m') p with
-    | Some v => VInt v
-    | None => VNil
+Fixpoint compile_concrete (p : Program) (m : ConcreteMState) : Check_T ConcreteMState :=
+  match p with
+  | [] => Legal m
+  | x :: xs =>
+    match apply_concrete x m with
+    | Legal m' => compile_concrete xs m'
+    | Illegal => Illegal
     end
-  ) (out_mem o) in
-  (reg_vals, mem_vals).
+  end.
 
-Definition programs_eq (p1 p2 : Program) (out : ProgramOutput) :=
-  forall (m : MachineState),
-  get_output p1 out m = get_output p2 out m.
-
-Definition TabulaRasa : MachineState := {|
-  reg_state := PMap.init VNil;
-  mem_state := PMap.init None
+Definition initial_state : ConcreteMState := {|
+  reg_state := PMap.init CrNil;
+  mem_state := @TabulaRasa CrVal;
 |}.
-
-Definition mx : MachineState := {|
-  reg_state := PMap.set 1 (VPtr (Address 0 0)) (PMap.init VNil);
-  mem_state := PMap.set (Pos.of_nat 1) (Some {|
-    base := 0;
-    len := 1024;
-    bytes := PMap.set 1 (Some (repr 10)) (PMap.init None)
-  |}) (PMap.init None)
-|}.
-
-Definition p1_v1 : Program := [
-  LdReg  (Reg 3) (Reg 1); (* r3 = *r1 *)
-  SetVal (Reg 6) (VInt (repr 10)); (* r6 = 10 *)
-  SetReg (Reg 7) (Reg 1); (* r7 = r1 *)
-  StReg  (Reg 7) (Reg 6); (* *r7 = r6 *)
-  SetReg (Reg 5) (Reg 1); (* r5 = r1 *)
-  LdReg  (Reg 4) (Reg 5); (* r4 = *r5 *)
-  AddReg (Reg 2) (Reg 3) (Reg 4) (* r2 = r3 + r4 *)
-].
-Definition p1_v2 : Program := [
-  LdReg  (Reg 2) (Reg 1); (* r2 = *r1 *)
-  AddVal (Reg 2) (Reg 2) (VInt (repr 10)) (* r2 = r2 + 10 *)
-].
-Definition p1_out : ProgramOutput := {|
-  out_reg := [Reg 2; Reg 17];
-  out_mem := [(Address 100 100)]
-|}.
-
-Definition check_registers_and_memory (s1 s2 : MachineState)
-  (out_list : ProgramOutput)
-
-Compute (get_output p1_v1 p1_out mx).
-Compute get_output p1_v2 p1_out mx.
-
-(* memory operators don't change register state *)
-Lemma alloc_is_regnop : forall base nbyte m,
-  reg_state (alloc base nbyte m) = reg_state m.
-Proof. intros. reflexivity. Qed.
-Lemma st_val_is_regnop : forall dst v m,
-  reg_state (st_val dst v m) = reg_state m.
-Proof. intros. unfold st_val. destruct ((reg_state m) !! (reg' dst)), v; reflexivity. Qed.
-Lemma st_reg_is_regnop : forall dst src m,
-  reg_state (st_reg dst src m) = reg_state m.
-Proof. intros. unfold st_reg. destruct ((reg_state m) !! (reg' dst)), ((reg_state m) !! (reg' src)); reflexivity. Qed.
-Lemma ist_reg_is_regnop : forall dst src m,
-  reg_state (ist_reg dst src m) = reg_state m.
-Proof. intros. unfold ist_reg. destruct ((reg_state m) !! (reg' dst)), ((reg_state m) !! (reg' src)); try reflexivity. destruct (ld_mem (mem_state m) p0); reflexivity. Qed.
-
-(* register operators don't change memory state *)
-Lemma set_val_is_memnop : forall dst v m,
-  mem_state (set_val dst v m) = mem_state m.
-Proof. intros. reflexivity. Qed.
-Lemma set_reg_is_memnop : forall dst src m,
-  mem_state (set_reg dst src m) = mem_state m.
-Proof. intros. reflexivity. Qed.
-Lemma ld_reg_is_memnop : forall dst src m,
-  mem_state (ld_reg dst src m) = mem_state m.
-Proof. intros. reflexivity. Qed.
-Lemma add_val_is_memnop : forall dst src v m,
-  mem_state (add_val dst src v m) = mem_state m.
-Proof. intros. reflexivity. Qed.
-Lemma add_reg_is_memnop : forall dst src1 src2 m,
-  mem_state (add_reg dst src1 src2 m) = mem_state m.
-Proof. intros. reflexivity. Qed.
-
-(* register operators don't affect other registers *)
-Lemma set_val_diff : forall r1 r2 v m,
-  r1 <> reg' r2 -> (reg_state (set_val r2 v m)) !! r1 = (reg_state m) !! r1.
-Proof. intros. simpl. rewrite PMap.gso; try reflexivity. assumption. Qed.
-Lemma set_reg_diff : forall r1 r2 src m,
-  r1 <> reg' r2 -> (reg_state (set_reg r2 src m)) !! r1 = (reg_state m) !! r1.
-Proof. intros. simpl. rewrite PMap.gso; try reflexivity. assumption. Qed.
-Lemma ld_reg_diff : forall r1 r2 src m,
-  r1 <> reg' r2 -> (reg_state (ld_reg r2 src m)) !! r1 = (reg_state m) !! r1.
-Proof. intros. simpl. rewrite PMap.gso; try reflexivity. assumption. Qed.
-Lemma add_val_diff : forall r1 r2 src v m,
-  r1 <> reg' r2 -> (reg_state (add_val r2 src v m)) !! r1 = (reg_state m) !! r1.
-Proof. intros. unfold add_val. apply set_val_diff. assumption. Qed.
-Lemma add_reg_diff : forall r1 r2 src1 src2 m,
-  r1 <> reg' r2 -> (reg_state (add_reg r2 src1 src2 m)) !! r1 = (reg_state m) !! r1.
-Proof. intros. unfold add_reg. apply set_val_diff. assumption. Qed.
-
-(* apply register operator *)
-Lemma ld_reg_same : forall r src m,
-  (reg_state (ld_reg (Reg r) src m)) !! r = x_reg m src.
-Proof.
-  intros. simpl. rewrite PMap.gss. reflexivity.
-Qed.
